% !TEX root =  ../main.tex

\subsection{Proof of Theorem~\ref{the:Rate} - Convergence Rate}
\label{sec:app:rate_single}

\theRate*

\begin{proof}
	Though the proof follows directly from Theorem~\ref{the:Repeat}, we also provide the following proof 
	for this simplified case as a stepping stone to aid in understanding the more general proof.
	
	Using Minkowski's inequality, we can bound the mean squared error of $I_{N,M}$ by
	\begin{align} \label{eq:mse-bound-app}\begin{split}
	\E[(I-I_{N,M})^2] &= \norm{I - I_{N,M}}_2^2 \leq {U}^2 + {V}^2 + 2 U V \leq 2\left(U^2 + V^2\right)
	\end{split}
	\end{align}
	\begin{eqnarray*}
		\text{where} \quad U = \norm{I - \frac{1}{N} \sum_{n=1}^N f(y_n, \gamma(y_n))}_2
		\quad \text{and} \quad
		V = \norm{\frac{1}{N} \sum_{n=1}^N f(y_n, \gamma(y_n)) - I_{N,M}}_2.
	\end{eqnarray*}
	We see immediately that $U = O\left(1 / \sqrt{N}\right)$, since $\frac{1}{N} \sum_{n=1}^N
	f(y_n, \gamma(y_n))$ is a MC estimator for $I$, noting our assumption that
	$f(y_n, \gamma(y_n)) \in L^2$. For the second term,
	\begin{eqnarray*}
		V &=& \norm{\frac{1}{N} \sum_{n=1}^N f(y_n, (\hat{\gamma}_M)_n) - f(y_n, \gamma(y_n))}_2 \\
		&\leq& \frac{1}{N} \sum_{n=1}^{N} \norm{f(y_n, (\hat{\gamma}_M)_n) - f(y_n,
			\gamma(y_n))}_2
		\leq \frac{1}{N} \sum_{n=1}^N K \norm{(\hat{\gamma}_M)_n - \gamma(y_n)}_2 \\
	\end{eqnarray*}
	where $K$ is a fixed constant, again by Minkowski and using the assumption that $f$ is
	Lipschitz. We can rewrite
	\[
	\norm{(\hat{\gamma}_M)_n - \gamma(y_n)}_2^2
	= \E \left[ \E \left[ ((\hat{\gamma}_M)_n - \gamma(y_n))^2 \middle| y_n \right]\right].
	\]
	by the tower property of conditional expectation, and note that
	\begin{align*}
	\E &\left[ ((\hat{\gamma}_M)_n - \gamma(y_n))^2 \middle| y_n \right]
	= \var\left(\frac{1}{M} \sum_{m=1}^M \phi(y_n, z_{n,m}) \middle| y_n \right) 
	= \frac{1}{M} \var\left(\phi(y_n, z_{n,1}) \middle| y_n \right)
	%    &=& \E_{y_n \sim p(y)} \left[ O(1/M) \right] \\
	%    &=& O(1/M),
	\end{align*}
	since each $z_{n,m}$ is i.i.d. and conditionally independent given $y_n$. As
	such
	\begin{align*}
	\norm{(\hat{\gamma}_M)_n - \gamma(y_n)}_2^2
	&= \frac{1}{M} \, \E \left[ \var \left(\phi(y_n, z_{n,1}) \middle| y_n \right)\right] 
	= O(1/M),
	\end{align*}
	noting that $\E \left[ \var \left(\phi(y_n, z_{n,1}) \middle| y_n \right)\right]$ is a
	finite constant by our assumption that $\phi(y_n, z_{n,m}) \in L^2$. Consequently,
	\[
	V \leq \frac{NK}{N} O\left(1/\sqrt{M}\right) = O\left(1/\sqrt{M}\right).
	\]
	Substituting these bounds for $U$ and $V$ in \eqref{eq:mse-bound-app} gives
	\begin{align*}
	\norm{I - I_{N,M}}_2^2
	&\leq 2\left(O\left(1/\sqrt{N}\right)^2 + O\left(1/\sqrt{M}\right)^2\right) 
	= O\left(1/N + 1/M\right)
	\end{align*}
	as desired.
\end{proof}